WIP connected components

dataplane/Examples/ConnectedComponents.thy
@@ -2,6 +2,7 @@ theory ConnectedComponents
 
 imports
   Accumulator
+  Input_top
   Dataplane.Timely_Infrastructure
 begin
 
@@ -47,23 +48,20 @@ instance ..
 end
 
 abbreviation cc_spec where
-  \<open>cc_spec \<equiv> accumulator_op (\<lambda>_. (\<union>)) (\<lambda>_. The \<circ> is_ccs) (\<lambda>_. 0)\<close>
+  \<open>cc_spec \<equiv> accumulator_op (\<lambda>_. (\<union>)) (\<lambda>_. The \<circ> is_ccs) (\<lambda>_. (=) {}) (\<lambda>_. 0)\<close>
 
 (* TODO move *)
-abbreviation "send_output op p x \<equiv> Write op (Some p) (Inr x)"
-abbreviation "send_progress op st \<equiv> Write op None (Inl (Inl st))"
-abbreviation "obtain_progress os \<equiv> (os\<lparr> consu := [], inter := [], produ := [] \<rparr>, \<lparr> cons = consu os, inte = inter os, prod = produ os\<rparr>)"
-abbreviation "drop_cap os cap \<equiv> (os\<lparr> inter := inter os @ [(out cap, time cap, -1)] \<rparr>)"
 abbreviation "mint_cap os p t \<equiv> os\<lparr> inter := inter os @ [(p, t, 1)] \<rparr>"
 abbreviation "produces os batch \<equiv> os\<lparr> outpu := (\<lambda> p. outpu os p @ map (\<lambda> (x, cap). (x, time cap)) (filter (\<lambda> (x, cap). out cap = p) batch)), produ := produ os @ map (\<lambda> (x, cap). (out cap, time cap, 1)) batch \<rparr>"
 
+(*
 (* Why use the Silent constructor? Is it to make it easier to reason later about the different possible steps? *)
 corec ooo_input_top where
   \<open>ooo_input_top os caps inps = choice3
   (Choice (cimage (\<lambda>p. case inps p of
     LCons (Data ts d) lxs \<Rightarrow>
       let cap = Cap (caps p) p;
-          os' = delay_cap os cap ts;
+          os' = if lxs = LNil then drop_cap os cap else delay_cap os cap ts;
           os'' = produce os' (Cap (time cap + ts) p) [d]
       in Silent (ooo_input_top os'' caps (inps(p := lxs)))
   | LCons (Watermark ts) lxs \<Rightarrow>
@@ -76,70 +74,101 @@ corec ooo_input_top where
     (cfilter (\<lambda>p. outpu os p \<noteq> []) c\<UU>)))
   (let (os', st) = obtain_progress os
   in send_progress (ooo_input_top os' caps inps) st)\<close>
+*)
 
 abbreviation \<open>choice4 op1 op2 op3 op4 \<equiv> choice2 (choice3 op1 op2 op3) op4\<close>
 abbreviation \<open>choice5 op1 op2 op3 op4 op5 \<equiv> choice2 (choice4 op1 op2 op3 op4) op5\<close>
 abbreviation \<open>choice6 op1 op2 op3 op4 op5 op6 \<equiv> choice2 (choice5 op1 op2 op3 op4 op5) op6\<close>
 abbreviation \<open>choice7 op1 op2 op3 op4 op5 op6 op7 \<equiv> choice2 (choice6 op1 op2 op3 op4 op5 op6) op7\<close>
 
-(* Should this operator use the frontier, or just do +(0, 1) on timestamps without caring? *)
 corec plus01_op where
-  \<open>plus01_op os caps = choice4
-  (Read None (\<lambda>st. case st of Inl (Inr f) \<Rightarrow> plus01_op (os\<lparr> front := f \<rparr>) caps | _ \<Rightarrow> \<oslash>))
+  \<open>plus01_op os = choice3
   (Choice (cimage (\<lambda>p. Read (Some p) (\<lambda>x. case x of
     Inr (d, ts) \<Rightarrow>
       let cap = Cap ts p;
-          (caps', os') = if cap \<in> set caps then (caps, os) else (caps @ [cap], mint_cap os p ts);
-          os'' = delay_cap os' cap (0, 1);
-          os''' = produce os'' (Cap (time cap + (0, 1)) p) [d]
-      in plus01_op os''' caps'
+          os' = consume os p ts 1;
+          os'' = produce os' (Cap (time cap + (0, 1)) p) [d]
+      in plus01_op os''
   | _ \<Rightarrow> \<oslash>)) c\<UU>))
   (Choice (cimage (\<lambda>p. case outpu os p of
-    x # xs \<Rightarrow> send_output (plus01_op (os\<lparr> outpu := (outpu os)(p := xs) \<rparr>) caps) p x)
+    x # xs \<Rightarrow> send_output (plus01_op (os\<lparr> outpu := (outpu os)(p := xs) \<rparr>)) p x)
     (cfilter (\<lambda>p. outpu os p \<noteq> []) c\<UU>)))
   (let (os', st) = obtain_progress os
-  in send_progress (plus01_op os' caps) st)\<close>
+  in send_progress (plus01_op os') st)\<close>
+
+lemma step_plus01_op_Inp_elim:
+  assumes \<open>step io (plus01_op os) op\<close>
+  obtains p d ts where \<open>io = Inp (Some p) (Inr (d, ts))\<close> \<open>op = plus01_op (produce (consume os p ts 1) (Cap (ts + (0, 1)) p) [d])\<close>
+  | p x where \<open>io = Inp (Some p) (Inl x)\<close> \<open>op = \<oslash>\<close>
+  | p x xs where \<open>io = Out (Some p) (Inr x)\<close> \<open>outpu os p = x # xs\<close> \<open>op = plus01_op (os\<lparr> outpu := (outpu os)(p := xs) \<rparr>)\<close>
+  | os' st where \<open>io = Out None (Inl (Inl st))\<close> \<open>obtain_progress os = (os', st)\<close> \<open>op = plus01_op os'\<close>
+  apply atomize_elim
+  using assms
+  apply (subst (asm) plus01_op.code)
+  apply (cases io)
+  by (auto split: sum.splits list.splits)
+
+declare [[unify_search_bound = 100]]
 
 corec label_prop_op where
-  \<open>label_prop_op os caps buf1 E buf2 lbls = choice7
-  (Read None (\<lambda>st. case st of Inl (Inr f) \<Rightarrow> label_prop_op (os\<lparr> front := f \<rparr>) caps buf1 E buf2 lbls | _ \<Rightarrow> \<oslash>))
+  \<open>label_prop_op os caps buf1 E buf2 label = choice7
+  (Read None (\<lambda>st. case st of Inl (Inr f) \<Rightarrow> label_prop_op (os\<lparr> front := f \<rparr>) caps buf1 E buf2 label | _ \<Rightarrow> \<oslash>))
   (Read (Some (1 :: 2)) (\<lambda>x. case x of
     Inr ((s, d), ts) \<Rightarrow>
       let cap = Cap ts 1;
           (caps', os') = if cap \<in> set caps then (caps, os) else (caps @ [cap], mint_cap os 1 ts);
+          os'' = consume os' 1 ts 1;
           buf1' = buf1(ts := buf1 ts @ [(s, d), (d, s)])
-     in label_prop_op os' (sort_key time caps') buf1' E buf2 lbls
+     in label_prop_op os'' (sort_key time caps') buf1' E buf2 label
   | _ \<Rightarrow> \<oslash>))
   (Read (Some (2 :: 2)) (\<lambda>x. case x of
     Inr ((n, x), ts) \<Rightarrow>
       let cap = Cap ts 2;
           (caps', os') = if cap \<in> set caps then (caps, os) else (caps @ [cap], mint_cap os 2 ts);
+          os'' = consume os' 1 ts 1;
           buf2' = buf2(ts := buf2 ts @ [(n, x)])
-    in label_prop_op os' (sort_key time caps') buf1 E buf2' lbls
+    in label_prop_op os'' (sort_key time caps') buf1 E buf2' label
   | _ \<Rightarrow> \<oslash>))
   (case [cap \<leftarrow> caps. time_below_frontier (time cap) (front os 1) \<and> out cap = 1] of
-    [] \<Rightarrow> Silent (label_prop_op os caps buf1 E buf2 lbls)
+    [] \<Rightarrow> Silent (label_prop_op os caps buf1 E buf2 label)
   | cap # caps' \<Rightarrow>
       let ts = time cap;
           buf1' = buf1(ts := []);
           E' = E @ buf1 ts;
           vertices = remdups (map fst E' @ map snd E');
           neighbors = (\<lambda>x. remdups [snd e. e \<leftarrow> E', fst e = x]);
-          batch = [((n, the (lbls v)), cap). v \<leftarrow> vertices, n \<leftarrow> neighbors v];
+          batch = [((n, label v), cap). v \<leftarrow> vertices, n \<leftarrow> neighbors v];
           os' = produces os batch;
           os'' = drop_cap os' cap
-      in Silent (label_prop_op os'' caps' buf1' E' buf2 lbls))
+      in Silent (label_prop_op os'' caps' buf1' E' buf2 label))
   (case [cap \<leftarrow> caps. time_below_frontier (time cap) (front os 2) \<and> out cap = 2] of
-    [] \<Rightarrow> Silent (label_prop_op os caps buf1 E buf2 lbls)
+    [] \<Rightarrow> Silent (label_prop_op os caps buf1 E buf2 label)
   | cap # caps' \<Rightarrow>
       let ts = time cap;
           buf2' = buf2(ts := []);
-          vertices = remdups (map fst E @ map snd E)
-      in undefined)
+          vertices = remdups (map fst E @ map snd E);
+          neighbors = (\<lambda>x. remdups [snd e. e \<leftarrow> E, fst e = x]);
+          min_label = (\<lambda>n. Min (set [x. (n, x) \<leftarrow> buf2 ts]));
+          updated_vertices = [v. v \<leftarrow> vertices, min_label v < label v];
+          label' = foldl (\<lambda>f v. f(v := min_label v)) label updated_vertices;
+          batch = [((n, label' v), cap). v \<leftarrow> updated_vertices, n \<leftarrow> neighbors v];
+          os' = produces os batch;
+          os'' = drop_cap os' cap
+      in Silent (label_prop_op os'' caps' buf1 E buf2' label'))
   (Choice (cimage (\<lambda>p. case outpu os p of
-    x # xs \<Rightarrow> send_output (label_prop_op (os\<lparr> outpu := (outpu os)(p := xs) \<rparr>) caps buf1 E buf2 lbls) p x)
+    x # xs \<Rightarrow> send_output (label_prop_op (os\<lparr> outpu := (outpu os)(p := xs) \<rparr>) caps buf1 E buf2 label) p x)
     (cfilter (\<lambda>p. outpu os p \<noteq> []) c\<UU>)))
   (let (os', st) = obtain_progress os
-  in send_progress (label_prop_op os' caps buf1 E buf2 lbls) st)\<close>
+  in send_progress (label_prop_op os' caps buf1 E buf2 label) st)\<close>
+
+abbreviation inp_op where
+  \<open>inp_op os n ins \<equiv>
+  map_op (case_option (Inl (0 :: 2)) (\<lambda>p. Inr (0, p))) (case_option (Inl (0 :: 2)) (\<lambda>p. Inr (0, p)))
+  (input_top os n ins)\<close>
+
+abbreviation plus_op where
+  \<open>plus_op os \<equiv>
+  map_op (case_option (Inl (1 :: 2)) (\<lambda>p. Inr (1, p))) (case_option (Inl (1 :: 2)) (\<lambda>p. Inr (1, p)))
+  (plus01_op os)\<close>
 
 end
